Completed encoding / decoding theorems

examples/acl2/ml/fmap_encodeScript.sml
@@ -9,6 +9,7 @@
 (*
 load "finite_mapTheory";
 load "sortingTheory";
+load "translateTheory";
 quietdec := true;
 open finite_mapTheory sortingTheory pred_setTheory listTheory pred_setLib;
 quietdec := false;
@@ -32,8 +33,10 @@ open finite_mapTheory pred_setTheory listTheory pred_setLib sortingTheory;
 
 val _ = new_theory "fmap_encode";
 
-val IND_STEP_TAC = PAT_ASSUM ``!y. P ==> Q`` 
-    (MATCH_MP_TAC o CONV_RULE (REPEATC (DEPTH_CONV (RIGHT_IMP_FORALL_CONV ORELSEC AND_IMP_INTRO_CONV))));
+val PULL_CONV = REPEATC (DEPTH_CONV (RIGHT_IMP_FORALL_CONV ORELSEC AND_IMP_INTRO_CONV));
+val PULL_RULE = CONV_RULE PULL_CONV;
+
+val IND_STEP_TAC = PAT_ASSUM ``!y. P ==> Q`` (MATCH_MP_TAC o PULL_RULE);
 
 (*****************************************************************************)
 (* fold for finite maps                                                      *)
@@ -165,7 +168,7 @@ val not_fempty_eq = prove(``!x. ~(x = FEMPTY) = (?y. y IN FDOM x)``,
 
 val fcard_less = prove(``!y x. y IN FDOM x ==> FCARD (x \\ y) < FCARD x``,
     RW_TAC std_ss [FCARD_DEF, FDOM_DOMSUB, CARD_DELETE, FDOM_FINITE] THEN
-    METIS_TAC [CARD_EQ_0, DECIDE ``0 < a = ¬(a = 0)``, NOT_IN_EMPTY, FDOM_FINITE]);
+    METIS_TAC [CARD_EQ_0, DECIDE ``0 < a = ¬(a = 0:num)``, NOT_IN_EMPTY, FDOM_FINITE]);
 
 val uniql_rec = prove(``!x y. uniql x /\ ¬(?z. MEM (y,z) x) ==> (uniql ((y,z)::x))``,
     Induct THEN RW_TAC std_ss [uniql_def, MEM] THEN METIS_TAC []);
@@ -193,7 +196,7 @@ val EXISTS_MEM_M2L = prove(``!x a. (?y. MEM (a,y) (M2L x)) = a IN FDOM x``,
 (* `!x. uniql (M2L x)`                                                       *)
 (*****************************************************************************)
 
-val UNIQL_M2L = prove(``!x. uniql (M2L x)``,
+val UNIQL_M2L = store_thm("UNIQL_M2L", ``!x. uniql (M2L x)``,
     GEN_TAC THEN completeInduct_on `FCARD x` THEN RW_TAC std_ss [M2L_def] THEN
     ONCE_REWRITE_TAC [fold_def] THEN RW_TAC std_ss [uniql_empty,GSYM M2L_def] THEN
     MATCH_MP_TAC uniql_rec THEN  `x' IN FDOM x` by METIS_TAC [not_fempty_eq] THEN
@@ -276,6 +279,19 @@ val L2M_APPLY = store_thm("L2M_APPLY",
     METIS_TAC []);
 
 (*****************************************************************************)
+(* L2M_APPLY_MAP_EQ:                                                         *)
+(* `!x f g y. ONE_ONE f /\ (?z. MEM (y,z) x) ==>                             *)
+(*          (L2M (MAP (f ## g) x) ' (f y) = g (L2M x ' y))                   *)
+(*****************************************************************************)
+
+val L2M_APPLY_MAP_EQ = store_thm("L2M_APPLY_MAP_EQ",
+    ``!x f g y. ONE_ONE f /\ (?z. MEM (y,z) x) ==> (L2M (MAP (f ## g) x) ' (f y) = g (L2M x ' y))``,
+    Induct THEN NTAC 2 (RW_TAC std_ss [L2M, MAP, MEM,FAPPLY_FUPDATE_THM,pairTheory.PAIR_MAP]) THEN 
+    FULL_SIMP_TAC std_ss [] THEN
+    Cases_on `h` THEN RW_TAC std_ss [FAPPLY_FUPDATE_THM] THEN
+    METIS_TAC [pairTheory.FST,ONE_ONE_THM]);
+
+(*****************************************************************************)
 (* APPLY_L2M_M2L                                                             *)
 (* `y IN FDOM x ==> (L2M (M2L x) ' y = x ' y)`                               *)
 (*****************************************************************************)
@@ -294,8 +310,19 @@ val L2M_M2L = store_thm("L2M_M2L",
     REWRITE_TAC [GSYM SUBMAP_ANTISYM, SUBMAP_DEF, FDOM_L2M_M2L] THEN
     RW_TAC std_ss [APPLY_L2M_M2L]);
 
+(*****************************************************************************)
+(* SETEQ                                                                     *)
+(*****************************************************************************)
 
 val SETEQ_def = Define `SETEQ l1 l2 = !x. MEM x l1 = MEM x l2`;
+
+val SETEQ_TRANS = store_thm("SETEQ_TRANS",
+    ``!l1 l2 l3. SETEQ l1 l2 /\ SETEQ l2 l3 ==> SETEQ l1 l3``,
+    RW_TAC std_ss [SETEQ_def]);
+
+val SETEQ_SYM = store_thm("SETEQ_SYM",
+    ``!l. SETEQ l l``,
+    RW_TAC std_ss [SETEQ_def]);
 
 (*****************************************************************************)
 (* M2L_L2M_SETEQ:                                                            *)
@@ -305,13 +332,27 @@ val SETEQ_def = Define `SETEQ l1 l2 = !x. MEM x l1 = MEM x l2`;
 val lemma1 = prove(``!x y z. uniql (y::x) ==> !z. MEM (FST y,z) x ==> (z = SND y)``,
     REPEAT (Cases ORELSE GEN_TAC) THEN REWRITE_TAC [uniql_def,MEM] THEN METIS_TAC []);
 
-val M2L_L2M_SETEQ = prove(``!x. uniql x ==> SETEQ x (M2L (L2M x))``,
+val M2L_L2M_SETEQ = store_thm("M2L_L2M_SETEQ",
+    ``!x. uniql x ==> SETEQ x (M2L (L2M x))``,
     Induct THEN RW_TAC std_ss [L2M, M2L_def, fold_FEMPTY, SETEQ_def,MEM] THEN
     IMP_RES_TAC uniql_cons THEN
     Cases_on `x' = h` THEN Cases_on `MEM x' x` THEN Cases_on `x'` THEN
     RW_TAC std_ss [GSYM M2L_def,GSYM IN_LIST_TO_SET, SET_M2L_FUPDATE] THEN
     RW_TAC std_ss [IN_LIST_TO_SET, MEM, MEM_M2L, FDOM_DOMSUB, DOMSUB_FAPPLY_THM, IN_DELETE, FDOM_L2M, L2M_APPLY] THEN
     METIS_TAC [lemma1,pairTheory.PAIR, L2M_APPLY, uniql_def]);
+
+(*****************************************************************************)
+(* M2L_L2M_MAP_SETEQ:                                                        *)
+(* `!l f g. ONE_ONE f ==>                                                    *)
+(*          SETEQ (M2L (L2M (MAP (f ## g) l))) (MAP (f ## g) (M2L (L2M l)))` *)
+(*****************************************************************************)
+
+val M2L_L2M_MAP_SETEQ = store_thm("M2L_L2M_MAP_SETEQ",
+    ``!l f g. ONE_ONE f ==> SETEQ (M2L (L2M (MAP (f ## g) l))) (MAP (f ## g) (M2L (L2M l)))``,
+    RW_TAC std_ss [SETEQ_def] THEN EQ_TAC THEN Cases_on `x` THEN
+    RW_TAC std_ss [pairTheory.PAIR_MAP, MEM_MAP,pairTheory.EXISTS_PROD, MEM_M2L,FDOM_L2M] THEN
+    TRY (Q.EXISTS_TAC `p_1`) THEN RW_TAC std_ss [] THEN
+    METIS_TAC [L2M_APPLY_MAP_EQ]);
 
 (*****************************************************************************)
 (*                                                                           *)
@@ -321,17 +362,15 @@ val SORTSET_def = Define `SORTSET sort relation = sort relation o SET_TO_LIST o 
 val SORTEDSET_def = Define `SORTEDSET r l = SORTED r l /\ ALL_DISTINCT l`;
 val MAPSET_def = Define `MAPSET r l = SORTED r l /\ ALL_DISTINCT (MAP FST l)`;
 
+local
+val not = ``$~ : bool -> bool``;
+in
 val RFILTER_EQ_NIL = 
-    CONJ (REWRITE_RULE [] (AP_TERM ``$~`` (SPEC_ALL FILTER_NEQ_NIL)))
-         (CONV_RULE (REWRITE_CONV [] THENC LAND_CONV SYM_CONV) (AP_TERM ``$~`` (SPEC_ALL FILTER_NEQ_NIL)))
+    CONJ (REWRITE_RULE [] (AP_TERM not (SPEC_ALL FILTER_NEQ_NIL)))
+         (CONV_RULE (REWRITE_CONV [] THENC LAND_CONV SYM_CONV) (AP_TERM not (SPEC_ALL FILTER_NEQ_NIL)))
+end
 
-val ALL_DISTINCT_THM = prove(``!l. ALL_DISTINCT l = !x. MEM x l ==> (FILTER ($= x) l = [x])``,
-    Induct THEN RW_TAC std_ss [ALL_DISTINCT, MEM, FILTER] THEN
-    EQ_TAC THEN RW_TAC std_ss [RFILTER_EQ_NIL] THENL [
-      ALL_TAC,
-      PAT_ASSUM ``!y. P`` (MP_TAC o Q.SPEC `h`),
-      PAT_ASSUM ``!y. P`` (MP_TAC o Q.SPEC `x`)] THEN
-   RW_TAC std_ss [RFILTER_EQ_NIL] THEN METIS_TAC[]);
+val ALL_DISTINCT_THM = ALL_DISTINCT_FILTER;
 
 (*****************************************************************************)
 (* PERM_S2L_L2S:                                                             *)
@@ -352,7 +391,7 @@ val IN_FILTER_SET = prove(``!x y. FINITE x /\ y IN x ==> (FILTER ($= y) (SET_TO_
     Q.EXISTS_TAC `CARD (REST x)` THEN RW_TAC std_ss [FINITE_REST, REST_DEF, CARD_DELETE, CHOICE_DEF, IN_DELETE, GSYM arithmeticTheory.NOT_ZERO_LT_ZERO,CARD_EQ_0]);
 
 val NOT_IN_FILTER_SET = prove(``!x y. FINITE x /\ ~(y IN x) ==> (FILTER ($= y) (SET_TO_LIST x) = [])``,
-    RW_TAC std_ss [REWRITE_RULE [] (AP_TERM ``$~`` (SPEC_ALL FILTER_NEQ_NIL)), MEM_SET_TO_LIST]);
+    RW_TAC std_ss [REWRITE_RULE [] (AP_TERM ``$~:bool -> bool`` (SPEC_ALL FILTER_NEQ_NIL)), MEM_SET_TO_LIST]);
 
 val FILTER_SET = store_thm("FILTER_SET",
     ``!x. FINITE x ==> (!y. FILTER ($= y) (SET_TO_LIST x) = if y IN x then [y] else [])``,
@@ -368,39 +407,50 @@ val NO_MEM_EMPTY = prove(``!l. (!x. ¬(MEM x l)) = (l = [])``,
 val SORTED_APPEND = prove(``!a b r. transitive r /\ SORTED r (a ++ b) ==> !x y. MEM x a /\ MEM y b ==> r x y``,
     Induct THEN METIS_TAC [APPEND,MEM,SORTED_EQ,MEM_APPEND]);
 
-val MEM_PERM = prove(``!l1 l2. PERM l1 l2 ==> (!a. MEM a l1 = MEM a l2)``,
+val MEM_PERM = store_thm("MEM_PERM", 
+    ``!l1 l2. PERM l1 l2 ==> (!a. MEM a l1 = MEM a l2)``,
     METIS_TAC [Q.SPEC `$= a` MEM_FILTER, PERM_DEF]);
 
 val PERM_SORTED_EQ = store_thm("PERM_SORTED_EQ",
-    ``!l1 l2 r. antisymmetric r /\ transitive r /\ PERM l1 l2 /\ SORTED r l1 /\ SORTED r l2 ==> (l1 = l2)``,
+    ``!l1 l2 r. (irreflexive r \/ antisymmetric r) /\ transitive r /\ PERM l1 l2 /\ SORTED r l1 /\ SORTED r l2 ==> (l1 = l2)``,
     REPEAT GEN_TAC THEN completeInduct_on `LENGTH l1 + LENGTH l2` THEN REPEAT Cases THEN REWRITE_TAC [LENGTH] THEN
     TRY (REWRITE_TAC [PERM_DEF, RFILTER_EQ_NIL, FILTER] THEN METIS_TAC [NOT_NIL_CONS]) THEN
     RW_TAC std_ss [NO_MEM_EMPTY] THEN
-    `t = t'` by PAT_ASSUM ``!y. P ==> q`` (MATCH_MP_TAC o CONV_RULE (REPEATC (DEPTH_CONV (RIGHT_IMP_FORALL_CONV ORELSEC AND_IMP_INTRO_CONV)))) THEN
+    `t' = t''` by IND_STEP_TAC THEN
     IMP_RES_TAC SORTED_EQ THEN RW_TAC arith_ss [] THEN
     FULL_SIMP_TAC std_ss [PERM_CONS_EQ_APPEND] THEN
     Cases_on `M` THEN FULL_SIMP_TAC std_ss [APPEND,list_11] THEN
     REPEAT (PAT_ASSUM ``a = b`` SUBST_ALL_TAC) THEN
-    `h = h''` by METIS_TAC [MEM_PERM, MEM, MEM_APPEND, SORTED_APPEND, relationTheory.antisymmetric_def] THEN
-    METIS_TAC [PERM_FUN_APPEND_CONS, PERM_TRANS, PERM_SYM, APPEND]);
+    METIS_TAC [MEM_PERM, MEM, MEM_APPEND, SORTED_APPEND, 
+    	       relationTheory.antisymmetric_def, relationTheory.irreflexive_def, relationTheory.transitive_def,
+    	       PERM_FUN_APPEND_CONS, PERM_TRANS, PERM_SYM, APPEND]);
 
 val SORTSET_SORTEDSET = store_thm("SORTSET_SORTEDSET",
-    ``!l. transitive R /\ antisymmetric R /\ SORTS sort R /\ SORTEDSET R l ==> (SORTSET sort R l = l)``,
+    ``!l. transitive R /\ (irreflexive R \/ antisymmetric R) /\ SORTS sort R /\ SORTEDSET R l ==> (SORTSET sort R l = l)``,
     RW_TAC std_ss [SORTEDSET_def,SORTSET_def, SETEQ_def, SORTS_DEF] THEN
     `PERM (sort R (SET_TO_LIST (set l))) l` by METIS_TAC [PERM_SYM, PERM_TRANS, PERM_S2L_L2S] THEN
     METIS_TAC [PERM_SORTED_EQ]);
 
-val ALL_DISTINCT_M2L = prove(``!s. ALL_DISTINCT (M2L s)``,
+val ALL_DISTINCT_M2L = store_thm("ALL_DISTINCT_M2L",
+    ``!s. ALL_DISTINCT (M2L s)``,
     completeInduct_on `FCARD s` THEN REPEAT STRIP_TAC THEN
     REWRITE_TAC [M2L_def] THEN ONCE_REWRITE_TAC [fold_def] THEN
     NTAC 2 (RW_TAC std_ss [ALL_DISTINCT, GSYM M2L_def,MEM_M2L,FDOM_DOMSUB,IN_DELETE]) THEN
     IND_STEP_TAC THEN
     METIS_TAC [fcard_less, not_fempty_eq]);
 
+val ALL_DISTINCT_MAPFST_M2L = store_thm("ALL_DISTINCT_MAPFST_M2L",
+    ``!s. ALL_DISTINCT (MAP FST (M2L s))``,
+    completeInduct_on `FCARD s` THEN REPEAT STRIP_TAC THEN
+    REWRITE_TAC [M2L_def] THEN ONCE_REWRITE_TAC [fold_def] THEN
+    NTAC 2 (RW_TAC std_ss [ALL_DISTINCT, GSYM M2L_def,MEM_M2L,FDOM_DOMSUB,IN_DELETE,MAP,MEM_MAP]) THEN
+    (IND_STEP_TAC ORELSE Cases_on `y` THEN RW_TAC std_ss [ALL_DISTINCT, GSYM M2L_def,MEM_M2L,FDOM_DOMSUB,IN_DELETE,MAP,MEM_MAP]) THEN
+    METIS_TAC [fcard_less, not_fempty_eq]);
+
 val PERM_DISTINCT = prove(``!l1 l2. PERM l1 l2 ==> (ALL_DISTINCT l1 = ALL_DISTINCT l2)``,
     METIS_TAC [MEM_PERM, PERM_DEF, ALL_DISTINCT_THM]);
 
-val SORTSET_SORT = prove(``!l R. antisymmetric R /\ transitive R /\ SORTS sort R /\ ALL_DISTINCT l ==> (SORTSET sort R l = sort R l)``,
+val SORTSET_SORT = prove(``!l R. (antisymmetric R \/ irreflexive R) /\ transitive R /\ SORTS sort R /\ ALL_DISTINCT l ==> (SORTSET sort R l = sort R l)``,
     RW_TAC std_ss [SORTS_DEF,SORTSET_def] THEN
     `PERM l (sort R (SET_TO_LIST (set l)))` by METIS_TAC [PERM_S2L_L2S, PERM_DISTINCT, PERM_TRANS, PERM_SYM] THEN
     MATCH_MP_TAC PERM_SORTED_EQ THEN RW_TAC std_ss [] THEN
@@ -410,12 +460,17 @@ val SORTSET_SORT = prove(``!l R. antisymmetric R /\ transitive R /\ SORTS sort R
 val PERM_S2L_L2S_EQ = prove(``!l1 l2. SETEQ l1 l2 ==> PERM (SET_TO_LIST (set l1)) (SET_TO_LIST (set l2))``,
     RW_TAC std_ss [PERM_DEF, FILTER_SET, FINITE_LIST_TO_SET,IN_LIST_TO_SET,SETEQ_def]);
 
-val PERM_SETEQ = prove(``!l1 l2. PERM l1 l2 ==> SETEQ l1 l2``,
+val PERM_SETEQ = store_thm("PERM_SETEQ",
+    ``!l1 l2. PERM l1 l2 ==> SETEQ l1 l2``,
     Induct THEN RW_TAC std_ss [PERM_CONS_EQ_APPEND, PERM_NIL,SETEQ_def] THEN
     Cases_on `x = h` THEN ASM_REWRITE_TAC [MEM, MEM_APPEND] THEN EQ_TAC THEN
     RES_TAC THEN FULL_SIMP_TAC std_ss [SETEQ_def, MEM_APPEND]);
 
-val SORTSET_EQ = prove(``!l1 l2 R. SORTS sort R /\ antisymmetric R /\ transitive R /\ SETEQ l1 l2 ==> (SORTSET sort R l1 = SORTSET sort R l2)``,
+val SETEQ_THM = store_thm("SETEQ_THM",
+    ``!l1 l2. SETEQ l1 l2 = (set l1 = set l2)``,
+    RW_TAC std_ss [pred_setTheory.EXTENSION, SETEQ_def, IN_LIST_TO_SET]);
+
+val SORTSET_EQ = prove(``!l1 l2 R. SORTS sort R /\ (irreflexive R \/ antisymmetric R) /\ transitive R /\ SETEQ l1 l2 ==> (SORTSET sort R l1 = SORTSET sort R l2)``,
     RW_TAC std_ss [SORTSET_def, SORTS_DEF] THEN
     MATCH_MP_TAC PERM_SORTED_EQ THEN Q.EXISTS_TAC `R` THEN RW_TAC std_ss [] THEN
     METIS_TAC [PERM_S2L_L2S_EQ,PERM_TRANS,PERM_SYM, PERM_SETEQ]);
@@ -431,8 +486,8 @@ val MAPSET_CONS = prove(``!a b R. MAPSET R (a::b) ==> MAPSET R b``,
     RW_TAC std_ss [MAPSET_def, MAP, ALL_DISTINCT, SORTED_CONS] THEN
     METIS_TAC [SORTED_CONS]);
 
-
-val MAPSET_UNIQ = prove(``!a R. MAPSET R a ==> uniql a``,	
+val MAPSET_UNIQ = store_thm("MAPSET_UNIQ",
+    ``!a R. MAPSET R a ==> uniql a``,	
     Induct THEN REPEAT STRIP_TAC THEN IMP_RES_TAC MAPSET_CONS THEN RES_TAC THEN
     FULL_SIMP_TAC std_ss [uniql_def, MEM, uniql_def, MAPSET_def, MAP, ALL_DISTINCT, MEM_MAP] THEN
     Cases_on `h` THEN RW_TAC std_ss [] THENL [
@@ -441,20 +496,608 @@ val MAPSET_UNIQ = prove(``!a R. MAPSET R a ==> uniql a``,
        ALL_TAC] THEN 
     ASM_REWRITE_TAC [] THEN METIS_TAC []);
 
+val ALL_DISTINCT_MAPFST = store_thm("ALL_DISTINCT_MAPFST",
+    ``!l. ALL_DISTINCT (MAP FST l) ==> ALL_DISTINCT l``,
+    Induct THEN RW_TAC std_ss [ALL_DISTINCT,MAP,MEM_MAP] THEN
+    METIS_TAC []);
+
+val MAPSET_DISTINCT = store_thm("MAPSET_DISTINCT",
+    ``MAPSET R x ==> ALL_DISTINCT x``,
+    METIS_TAC [MAPSET_def,ALL_DISTINCT_MAPFST]);
+
+val TOTAL_LEX = prove(``!R R'. total R /\ total R' ==> total (R LEX R')``,
+    RW_TAC std_ss [pairTheory.LEX_DEF,relationTheory.total_def] THEN
+    Cases_on `x` THEN Cases_on `y` THEN RW_TAC std_ss [] THEN
+    METIS_TAC []);
+
+val TRANSITIVE_LEX = store_thm("TRANSITIVE_LEX",
+    ``!R R'. transitive R /\ transitive R' ==> transitive (R LEX R')``,
+    RW_TAC std_ss [pairTheory.LEX_DEF,relationTheory.transitive_def] THEN
+    Cases_on `x` THEN Cases_on `y` THEN Cases_on `z` THEN RW_TAC std_ss [] THEN
+    FULL_SIMP_TAC std_ss [] THEN
+    METIS_TAC []);
+
+val SORTED_LEX = store_thm("SORTED_LEX",
+    ``!R1 R2. total R1 /\ transitive R1 /\ transitive R2 ==> !x. SORTED (R1 LEX R2) x ==> SORTED R1 (MAP FST x)``,
+    NTAC 3 STRIP_TAC THEN Induct THEN TRY Cases THEN RW_TAC std_ss [SORTED_EQ,MAP,SORTED_DEF,TRANSITIVE_LEX,MEM_MAP,pairTheory.LEX_DEF] THEN
+    RES_TAC THEN Cases_on `y'` THEN FULL_SIMP_TAC std_ss [] THEN
+    METIS_TAC [relationTheory.transitive_def, relationTheory.total_def]);
+
+val filter_first = prove(``!l x y. (FILTER ($= x) (MAP FST l) = [x]) /\ (x = FST y) /\ MEM y l ==> (FILTER ($= x o FST) l = [y])``,
+    Induct THEN RW_TAC std_ss [FILTER,MEM,RFILTER_EQ_NIL] THEN
+    FULL_SIMP_TAC std_ss [MAP,FILTER,list_11,RFILTER_EQ_NIL, MEM_MAP] THEN
+    FIRST [PAT_ASSUM ``a = b`` MP_TAC, METIS_TAC []] THEN
+    RW_TAC std_ss [RFILTER_EQ_NIL, MEM_MAP] THEN METIS_TAC []);
+
+val MAP_FST_DISTINCT_EQ = store_thm("MAP_FIRST_DISTINCT_EQ",
+    ``!l1 l2. (MAP FST l1 = MAP FST l2) /\ ALL_DISTINCT (MAP FST l1) /\ PERM l1 l2 ==> (l1 = l2)``,
+    REPEAT STRIP_TAC THEN MATCH_MP_TAC LIST_EQ THEN RW_TAC std_ss [PERM_LENGTH,pairTheory.PAIR_FST_SND_EQ] THEN
+    `FST (EL x l1) = FST (EL x l2)` by METIS_TAC [EL_MAP, PERM_LENGTH] THEN
+    FULL_SIMP_TAC std_ss [ALL_DISTINCT_FILTER] THEN
+    `MEM (FST (EL x l2)) (MAP FST l2) /\ MEM (FST (EL x l1)) (MAP FST l1)` by METIS_TAC [MEM_MAP, rich_listTheory.EL_IS_EL,PERM_LENGTH] THEN
+    MAP_EVERY (fn x => x by (MATCH_MP_TAC filter_first THEN METIS_TAC [filter_first, rich_listTheory.EL_IS_EL, PERM_LENGTH, MEM_PERM])) [
+         `FILTER ($= (FST (EL x l2)) o FST) l2 = [EL x l2]`,
+         `FILTER ($= (FST (EL x l2)) o FST) l2 = [EL x l1]`] THEN
+    METIS_TAC [pairTheory.PAIR,list_11]);
+
+
+val SETEQ_PERM = store_thm("SETEQ_PERM",
+    ``!l1 l2. SETEQ l1 l2 /\ ALL_DISTINCT l1 /\ ALL_DISTINCT l2 ==> PERM l1 l2``,
+    RW_TAC std_ss [SETEQ_def, ALL_DISTINCT_FILTER, PERM_DEF] THEN
+    Cases_on `MEM x l1` THEN1 METIS_TAC [FILTER_NEQ_NIL] THEN
+    MAP_EVERY (fn x => x by RW_TAC std_ss [RFILTER_EQ_NIL])
+         [`FILTER ($= x) l1 = []`, `FILTER ($= x) l2 = []`] THEN
+    METIS_TAC []);
 
 (*****************************************************************************)
 (* M2L_L2M:                                                                  *)
-(*`!l sort R. transitive R /\ antisymmetric R /\                             *) 
-(*            SORTS sort R /\ MAPSET R l ==> (sort R (M2L (L2M l)) = l)`     *)
+(*`!R R' sort. total R /\ transitive R /\ transitive R' /\ antisymmetric R   *)
+(*               /\ SORTS sort (R LEX R')                                    *)
+(*               ==> !l. MAPSET (R LEX R') l                                 *)
+(*                       ==> (sort (R LEX R') (M2L (L2M l)) = l)`            *)
 (*****************************************************************************)
 
-val M2L_L2M = store_thm("M2L_L2M",
-    ``!l sort R. transitive R /\ antisymmetric R /\ SORTS sort R /\ MAPSET R l ==> (sort R (M2L (L2M l)) = l)``,
+val M2L_L2M = store_thm("M2L_L2M", 
+    ``!sort R R'. total R /\ antisymmetric R /\ transitive R /\ transitive R' /\ 
+                    SORTS sort (R LEX R') ==> !l. MAPSET (R LEX R') l 
+                    ==> (sort (R LEX R') (M2L (L2M l)) = l)``,
     REPEAT STRIP_TAC THEN
-    `(sort R (M2L (L2M l)) = l) = (SORTSET sort R (M2L (L2M l)) = SORTSET sort R l)` by 
-    	   METIS_TAC [ALL_DISTINCT_M2L, SORTSET_SORT, SORTSET_SORTEDSET, MAPSET_IMP_SORTEDSET] THEN
-    ASM_REWRITE_TAC [] THEN MATCH_MP_TAC SORTSET_EQ THEN ASM_REWRITE_TAC [] THEN
-    METIS_TAC [SETEQ_def, M2L_L2M_SETEQ, MAPSET_UNIQ]);
+    CONV_TAC SYM_CONV THEN MATCH_MP_TAC MAP_FST_DISTINCT_EQ THEN
+    IMP_RES_TAC MAPSET_def THEN
+    REPEAT STRIP_TAC THEN FULL_SIMP_TAC std_ss [SORTS_DEF] THEN
+    TRY (
+        MATCH_MP_TAC PERM_SORTED_EQ THEN Q.EXISTS_TAC `R` THEN REPEAT CONJ_TAC THEN TRY (MATCH_MP_TAC (PULL_RULE SORTED_LEX) THEN METIS_TAC []) THEN
+        ASM_REWRITE_TAC [] THEN MATCH_MP_TAC PERM_MAP) THEN
+    MATCH_MP_TAC SETEQ_PERM THEN
+    RW_TAC std_ss [ALL_DISTINCT_MAPFST] THEN 
+    REPEAT (MAP_FIRST MATCH_MP_TAC [PERM_SETEQ, PERM_TRANS]) THEN
+    TRY (Q.EXISTS_TAC `M2L (L2M l)`) THEN RW_TAC std_ss [] THEN
+    TRY (MATCH_MP_TAC SETEQ_PERM) THEN 
+    METIS_TAC [M2L_L2M_SETEQ, MAPSET_UNIQ, ALL_DISTINCT_PERM, ALL_DISTINCT_M2L, ALL_DISTINCT_MAPFST]);   
+
+(*****************************************************************************)
+(* SEXP Ordering theorems                                                    *)
+(*****************************************************************************)
+
+val SEXP_LT_def = Define `
+    (SEXP_LT (sym a0 b0) (sym c0 d0) = a0 < c0 \/ (a0 = c0) /\ (b0 < d0)) /\
+    (SEXP_LT (sym a0 b0) _ = T) /\
+    (SEXP_LT (str a1) (str b1) = a1 < b1) /\
+    (SEXP_LT (str a1) (sym a0 b0) = F) /\
+    (SEXP_LT (str a1) _ = T) /\
+    (SEXP_LT (chr a2) (chr b2) = a2 < b2) /\
+    (SEXP_LT (chr a2) (sym a0 b0) = F) /\
+    (SEXP_LT (chr a2) (str a1) = F) /\
+    (SEXP_LT (chr a2) _ = T) /\
+    (SEXP_LT (num a3) (num b3) = a3 < b3) /\
+    (SEXP_LT (num a3) (sym a0 b0) = F) /\
+    (SEXP_LT (num a3) (str a1) = F) /\
+    (SEXP_LT (num a3) (chr a2) = F) /\
+    (SEXP_LT (num a3) (cons a b) = T) /\
+    (SEXP_LT (cons a4 b4) (cons c4 d4) = SEXP_LT a4 c4 \/ (a4 = c4) /\ SEXP_LT b4 d4) /\
+    (SEXP_LT (cons a4 b4) _ = F)`;
+
+val _ = overload_on ("<", ``SEXP_LT``);
+
+
+val TRANS_INV = store_thm("TRANS_INV",
+    ``!R f. transitive R ==> transitive (inv_image R f)``,
+    RW_TAC std_ss [relationTheory.transitive_def,relationTheory.inv_image_def] THEN
+    METIS_TAC []);
+
+val TOTAL_INV = store_thm("TOTAL_INV",
+    ``!R f. total R ==> total (inv_image R f)``,
+    RW_TAC std_ss [relationTheory.total_def,relationTheory.inv_image_def] THEN
+    METIS_TAC []);    
+
+val IRREFL_INV = store_thm("IRREFL_INV",
+    ``!R f. irreflexive R ==> irreflexive (inv_image R f)``,
+    RW_TAC std_ss [relationTheory.irreflexive_def,relationTheory.inv_image_def] THEN
+    METIS_TAC []);
+
+val ANTISYM_INV = store_thm("ANTISYM_INV",
+    ``!R f. ONE_ONE f /\ antisymmetric R ==> antisymmetric (inv_image R f)``,
+    RW_TAC std_ss [relationTheory.antisymmetric_def,relationTheory.inv_image_def, ONE_ONE_DEF]);
+
+val COM_LT_TRANS = prove(``!a b c. a < b /\ b < c ==> a < c : complex_rational``,
+    REPEAT Cases THEN RW_TAC std_ss [complex_rationalTheory.COMPLEX_LT_def] THEN
+    METIS_TAC [ratTheory.RAT_LES_TRANS]);
+
+val COM_LT_REFL = prove(``!a. ~(a < a : complex_rational)``,
+    REPEAT Cases THEN RW_TAC std_ss [complex_rationalTheory.COMPLEX_LT_def] THEN
+    METIS_TAC [ratTheory.RAT_LES_REF]);
+
+val COM_LT_TOTAL = prove(``!a b. a < b \/ b < a \/ (a = b : complex_rational)``,
+    REPEAT Cases THEN RW_TAC std_ss [complex_rationalTheory.COMPLEX_LT_def] THEN
+    METIS_TAC [ratTheory.RAT_LES_TOTAL]);
+
+val SEXP_LT_IRREFLEXIVE = prove(``irreflexive SEXP_LT``,
+    REWRITE_TAC [relationTheory.irreflexive_def] THEN
+    completeInduct_on `sexp_size x` THEN
+    Cases THEN REWRITE_TAC [SEXP_LT_def] THEN
+    TRY (METIS_TAC [stringTheory.string_lt_nonrefl, stringTheory.char_lt_def, prim_recTheory.LESS_REFL, COM_LT_REFL]) THEN
+    RW_TAC std_ss [sexpTheory.sexp_size_def] THEN IND_STEP_TAC THEN
+    RW_TAC arith_ss []);
+
+local
+val m = METIS_TAC [stringTheory.string_lt_trans,stringTheory.string_lt_nonrefl, arithmeticTheory.LESS_TRANS, stringTheory.char_lt_def, prim_recTheory.LESS_REFL, COM_LT_REFL, COM_LT_TRANS];
+in
+val order_lemma = prove(``!a b. ~(SEXP_LT a b /\ SEXP_LT b a)``,
+    completeInduct_on `sexp_size a + sexp_size b` THEN
+    NTAC 2 Cases THEN REWRITE_TAC [SEXP_LT_def] THENL [
+     m, m, m, m, ALL_TAC] THEN 
+    Cases_on `s = s'` THEN RW_TAC std_ss [sexpTheory.sexp_size_def, REWRITE_RULE [relationTheory.irreflexive_def] SEXP_LT_IRREFLEXIVE] THEN
+    FULL_SIMP_TAC std_ss [] THEN IND_STEP_TAC THEN
+    RW_TAC arith_ss [])
+end;
+
+local
+val m = METIS_TAC [stringTheory.string_lt_trans, stringTheory.char_lt_def, arithmeticTheory.LESS_TRANS, COM_LT_TRANS]
+in
+val SEXP_LT_TRANSITIVE = store_thm("SEXP_LT_TRANSITIVE",
+    ``transitive SEXP_LT``,
+    REWRITE_TAC [relationTheory.transitive_def] THEN
+    completeInduct_on `sexp_size x + sexp_size y + sexp_size z` THEN
+    NTAC 3 Cases THEN REWRITE_TAC [SEXP_LT_def] THENL [
+        m, m, m, m, ALL_TAC] THEN
+    RW_TAC std_ss [sexpTheory.sexp_size_def] THENL [
+      Cases_on `s = s''`, Cases_on `s = s'`, Cases_on `s = s''`, ALL_TAC] THEN
+    RW_TAC std_ss [REWRITE_RULE [relationTheory.irreflexive_def] SEXP_LT_IRREFLEXIVE] THEN
+    IND_STEP_TAC THEN RW_TAC std_ss [] THENL [
+      ALL_TAC, Q.EXISTS_TAC `s'`, Q.EXISTS_TAC `s0'`] THEN
+    RW_TAC arith_ss [] THEN METIS_TAC [order_lemma])
+end;
+
+val SEXP_LE_def = Define `SEXP_LE a b = (a = b) \/ SEXP_LT a b`;
+
+local
+val m = METIS_TAC [stringTheory.string_lt_cases, stringTheory.char_lt_def, arithmeticTheory.LESS_LESS_CASES, sexpTheory.sexp_11, stringTheory.ORD_11, COM_LT_TOTAL];
+in
+val SEXP_LE_TOTAL = prove(``total SEXP_LE``,
+    REWRITE_TAC [relationTheory.total_def] THEN
+    completeInduct_on `sexp_size x + sexp_size y` THEN
+    NTAC 2 Cases THEN REWRITE_TAC [SEXP_LE_def, SEXP_LT_def] THENL [
+     m, m, m, m, ALL_TAC] THEN RW_TAC std_ss [sexpTheory.sexp_size_def] THEN
+    `(SEXP_LE s s' \/ SEXP_LE s' s) /\ (SEXP_LE s0 s0' \/ SEXP_LE s0' s0)` by CONJ_TAC THEN TRY IND_STEP_TAC THEN RW_TAC arith_ss [] THEN
+    FULL_SIMP_TAC std_ss [SEXP_LE_def,SEXP_LT_def])
+end;
+
+val SEXP_LE_TRANSITIVE = store_thm("SEXP_LE_TRANSITIVE",
+    ``transitive SEXP_LE``,
+    REWRITE_TAC [relationTheory.transitive_def, SEXP_LE_def] THEN
+    METIS_TAC [REWRITE_RULE [relationTheory.transitive_def] SEXP_LT_TRANSITIVE]);
+
+val SEXP_LE_ANTISYMMETRIC = store_thm("SEXP_LE_ANTISYMMETRIC",
+    ``antisymmetric SEXP_LE``,
+    METIS_TAC [SEXP_LT_TRANSITIVE, SEXP_LT_IRREFLEXIVE, relationTheory.transitive_def, relationTheory.irreflexive_def, relationTheory.antisymmetric_def, SEXP_LE_def]);
+
+val _ = overload_on ("<=", ``SEXP_LE``);
+
+(*****************************************************************************)
+(* Stable sort proofs                                                        *)
+(* Creates 'MINSORT' - an O(n^2) sort that just puts the minimum at the      *)
+(* and proves that this is a stable sort.                                    *)
+(*****************************************************************************)
+
+val o_assoc = prove(``(a o b) o c = a o (b o c)``, METIS_TAC [combinTheory.o_DEF]);
+
+val STABLE_def = Define `
+    STABLE sort r = SORTS sort r /\ 
+                    !p. (!x y. p x /\ p y ==> r x y) ==> (!l. FILTER p l = FILTER p (sort r l))`;
+
+val MIN_def = Define `
+    (MIN r a [] = a) /\ 
+    (MIN r a (head::tail) = 
+             if r a head then MIN r a tail else MIN r head tail)`;
+
+val DROP_def = Define `
+    (DROP h [] = []) /\
+    (DROP h (a::b) = if (h = a) then b else a::DROP h b)`;
+
+val MIN_CASES = prove(``!l h R. (MIN R h l = h) \/ (MEM (MIN R h l) l)``,
+    Induct THEN RW_TAC std_ss [MIN_def,MEM] THEN METIS_TAC []);
+
+val MIN_MEM = prove(``!l h R. MEM (MIN R h l) (h :: l)``,
+    Induct THEN RW_TAC std_ss [MIN_def,MEM] THEN METIS_TAC [MEM]);
+
+val DROP_LT = prove(``!l h. MEM h l ==> (LENGTH (DROP h l) < LENGTH l)``,
+    Induct THEN RW_TAC arith_ss [DROP_def,MIN_def,LENGTH,MEM]);
+
+val MINSORT_def = TotalDefn.tDefine "MINSORT"
+    `(MINSORT r [] = []) /\ 
+     (MINSORT r (hd::tl) = MIN r hd tl :: MINSORT r (DROP (MIN r hd tl) (hd::tl)))`
+    (WF_REL_TAC `measure (LENGTH o SND)` THEN METIS_TAC [DROP_LT, MIN_MEM]);
+
+val EXISTS_MINIMUM = store_thm("EXISTS_MINIMUM",
+    ``!P l. EXISTS P l ==> ?h M N. MEM h l /\ P h /\ ~EXISTS P M /\ (l = M ++ h::N)``,
+    GEN_TAC THEN Induct THEN RW_TAC std_ss [EXISTS_DEF,NOT_EXISTS,EVERY_MEM, MEM] THEN Cases_on `P h` THEN RES_TAC THENL [
+      MAP_EVERY Q.EXISTS_TAC [`h`, `[]`, `l`], 
+      MAP_EVERY Q.EXISTS_TAC [`h`, `[]`, `l`], 
+      MAP_EVERY Q.EXISTS_TAC [`h'`, `h::M`, `N`]] THEN
+    RW_TAC std_ss [MEM,APPEND] THEN
+    FULL_SIMP_TAC std_ss [NOT_EXISTS, EVERY_MEM, APPEND, MEM_APPEND, EXISTS_APPEND]);
+
+val NOT_MEM_DROP = prove(``!l h. ~MEM h l ==> (DROP h l = l)``,
+    Induct THEN RW_TAC std_ss [MEM, DROP_def]);
+
+val DROP_APPEND = prove(``!M N h. DROP h (M ++ N) = if MEM h M then DROP h M ++ N else M ++ DROP h N``,
+    completeInduct_on `LENGTH (M ++ N)` THEN REPEAT Cases THEN
+    NTAC 2 (RW_TAC std_ss [DROP_def,APPEND,APPEND_NIL,LENGTH,MEM]) THEN FULL_SIMP_TAC std_ss [NOT_MEM_DROP]);
+
+val DROP_SPLIT = prove(``!h l. MEM h l ==> (?M N. (DROP h l = M ++ N) /\ ~MEM h M /\ (l = M ++ h::N))``,
+    REPEAT STRIP_TAC THEN `EXISTS ($= h) l` by RW_TAC std_ss [EXISTS_MEM] THEN
+    IMP_RES_TAC EXISTS_MINIMUM THEN
+    MAP_EVERY Q.EXISTS_TAC [`M`, `N`] THEN
+    RW_TAC std_ss [DROP_APPEND,DROP_def] THEN
+    FULL_SIMP_TAC std_ss [EXISTS_MEM]);
+
+val PERM_MINSORT = store_thm("PERM_MINSORT",
+    ``!l. PERM l (MINSORT R l)``,
+    completeInduct_on `LENGTH l` THEN Cases  THEN RW_TAC std_ss [MINSORT_def, PERM_NIL] THEN
+    STRIP_ASSUME_TAC (MATCH_MP DROP_SPLIT (Q.SPECL [`t'`, `h`, `R`] MIN_MEM)) THEN
+    ONCE_REWRITE_TAC [PERM_SYM] THEN RW_TAC std_ss [PERM_CONS_EQ_APPEND] THEN
+    MAP_EVERY Q.EXISTS_TAC [`M`, `N`] THEN
+    RW_TAC std_ss [] THEN ONCE_REWRITE_TAC [PERM_SYM] THEN IND_STEP_TAC THEN
+    METIS_TAC [DROP_LT, MIN_MEM]);
+
+val MEM_DROP_IMP = prove(``!l a y. MEM y (DROP a l) ==> MEM y l``,
+    Induct THEN RW_TAC std_ss [MEM, DROP_def] THEN
+    METIS_TAC [MEM]);
+
+val R_MIN = store_thm("R_MIN",
+    ``!R. total R /\ transitive R ==> !l h y. MEM y (h::l) ==> R (MIN R h l) y``,
+    NTAC 2 STRIP_TAC THEN Induct THEN RW_TAC std_ss [MEM, MIN_def] THEN
+    METIS_TAC [relationTheory.total_def, relationTheory.transitive_def, MEM]);
+
+val SORTS_MINSORT = store_thm("SORTS_MINSORT", 
+    ``!R. total R /\ transitive R ==> SORTS MINSORT R``,
+    RW_TAC std_ss [SORTS_DEF,SORTED_DEF, PERM_MINSORT, SORTED_DEF] THEN
+    completeInduct_on `LENGTH l` THEN Cases THEN
+    REVERSE (RW_TAC std_ss [MINSORT_def, SORTED_DEF, SORTED_EQ]) THEN1
+       METIS_TAC [MEM_DROP_IMP, PERM_MINSORT, MEM_PERM, R_MIN] THEN
+    STRIP_ASSUME_TAC (MATCH_MP DROP_SPLIT (Q.SPECL [`t'`, `h`, `R`] MIN_MEM)) THEN
+    RW_TAC std_ss [] THEN IND_STEP_TAC THEN
+    METIS_TAC [DROP_LT, MIN_MEM]);
+
+val TOTAL_K = prove(``total (K (K T))``, RW_TAC std_ss [relationTheory.total_def]);
+val TRANSITIVE_K = prove(``transitive (K (K T))``, RW_TAC std_ss [relationTheory.transitive_def]);
+
+val R_H_MIN = store_thm("R_H_MIN",
+    ``!l R h. transitive R /\ total R /\ R h (MIN R h l) ==> (h = MIN R h l)``,
+    Induct THEN RW_TAC std_ss [MIN_def] THEN
+    METIS_TAC [R_MIN, relationTheory.transitive_def, relationTheory.total_def]);
+
+val R_MIN_H = store_thm("R_MIN_H",
+    ``!l R h. transitive R /\ total R ==> R (MIN R h l) h``, 
+    Induct THEN RW_TAC std_ss [MIN_def] THEN
+    METIS_TAC [R_MIN, relationTheory.transitive_def, relationTheory.total_def]);
+
+val MIN_EQ_APPEND = store_thm("MIN_EQ_APPEND",
+    ``!M N R x. transitive R /\ total R /\ (x = MIN R x (M ++ N)) ==> (x = MIN R x M) /\ (x = MIN R x N)``,
+    Induct THEN RW_TAC std_ss [MIN_def, APPEND, MEM] THEN
+    METIS_TAC [R_H_MIN, relationTheory.transitive_def, relationTheory.total_def]);
+
+val MIN_MEM_APPEND_L = store_thm("MIN_MEM_APPEND_L",
+    ``!M N R x. transitive R /\ total R /\ MEM (MIN R x (M ++ N)) M ==> (MIN R x (M ++ N) = MIN R x M)``,
+    Induct THEN RW_TAC std_ss [MIN_def, APPEND, MEM] THEN
+    METIS_TAC [MIN_EQ_APPEND, R_H_MIN]);
+
+val MIN_EXISTS = prove(``!l hd. ~(hd = MIN R hd l) ==> EXISTS ($= (MIN R hd l)) l /\ MEM (MIN R hd l) l``,
+    Induct THEN RW_TAC std_ss [MIN_def, EXISTS_DEF, MEM] THEN METIS_TAC []);
+
+val ALL_MIN_SPLIT = store_thm("ALL_MIN_SPLIT", 
+    ``!l. ~(hd = MIN R hd l) ==> (?M N. (l = M ++ MIN R hd l :: N) /\ ~(MEM (MIN R hd l) M))``,
+   REPEAT STRIP_TAC THEN IMP_RES_TAC MIN_EXISTS THEN IMP_RES_TAC (Q.SPECL [`$= (MIN R hd l)`,`l`] EXISTS_MINIMUM) THEN
+   MAP_EVERY Q.EXISTS_TAC [`M`,`N`] THEN FULL_SIMP_TAC std_ss [NOT_EXISTS, EVERY_MEM] THEN
+   METIS_TAC []);
+
+val MIN_LEMMA1 = prove(``!R. transitive R /\ total R ==> !l x M N h. ~(MIN R x l = x) /\ ~MEM (MIN R x l) M /\ (l = M ++ MIN R x l:: N) /\ R x h ==> (MIN R x l = MIN R h l)``,
+    NTAC 2 STRIP_TAC THEN Induct THEN REPEAT (Cases ORELSE GEN_TAC) THEN RW_TAC std_ss [MIN_def,MEM,list_11,APPEND,APPEND_eq_NIL,EXISTS_DEF] THEN
+    Cases_on `R x h''` THEN FULL_SIMP_TAC std_ss [MIN_def] THEN
+    METIS_TAC [relationTheory.transitive_def, relationTheory.total_def, R_H_MIN, R_MIN_H, R_MIN]);
+
+val MIN_LEMMA2 = prove(``!R. transitive R /\ total R ==> !l x M. ~(MIN R x l = x) /\ ~MEM (MIN R x l) M /\ (l = M ++ MIN R x l::N) ==> !y. MEM y M ==> ~R y (MIN R x l)``,
+    NTAC 2 STRIP_TAC THEN Induct THEN REPEAT (Cases ORELSE GEN_TAC) THEN RW_TAC std_ss [MIN_def,MEM,list_11,APPEND,APPEND_eq_NIL,EXISTS_DEF] THEN
+    METIS_TAC [MIN_LEMMA1, R_H_MIN]);
+
+val DROP_FILTER = prove(``!l x p. ~p x ==> (FILTER p (DROP x l) = FILTER p l)``,
+    Induct THEN RW_TAC std_ss [FILTER,DROP_def]);
+
+val MINSORT_STABLE = store_thm("MINSORT_STABLE",
+    ``!R. transitive R /\ total R ==> STABLE MINSORT R``,
+    RW_TAC std_ss [STABLE_def, SORTS_MINSORT] THEN
+    CONV_TAC SYM_CONV THEN
+    completeInduct_on `LENGTH l` THEN Cases THEN
+    RW_TAC std_ss [FILTER, MINSORT_def, CONJUNCT1 LENGTH] THEN
+    TRY (`(h = MIN R h t')` by METIS_TAC [R_H_MIN, R_MIN, MIN_MEM] THEN FULL_SIMP_TAC std_ss [DROP_def, LENGTH]) THEN
+    `FILTER p (MINSORT R (DROP (MIN R h t') (h::t'))) = FILTER p (DROP (MIN R h t') (h::t'))` by IND_STEP_TAC THEN
+    RW_TAC std_ss [DROP_LT, MIN_MEM, DROP_FILTER, FILTER] THEN
+    STRIP_ASSUME_TAC (MATCH_MP DROP_SPLIT (Q.SPECL [`t'`, `h`, `R`] MIN_MEM)) THEN RW_TAC std_ss [] THEN
+    Cases_on `M` THEN FULL_SIMP_TAC std_ss [list_11, APPEND,MEM] THEN1 METIS_TAC [] THEN
+    `!x. MEM x t'' ==> ~R x (MIN R h t')` by METIS_TAC [MIN_LEMMA2] THEN
+    RW_TAC std_ss [rich_listTheory.FILTER_APPEND,FILTER] THEN
+    `FILTER p t'' = []` by (RW_TAC std_ss [FILTER_EQ_NIL, EVERY_MEM] THEN METIS_TAC []) THEN
+    RW_TAC std_ss [APPEND] THEN
+    PAT_ASSUM ``b = c ++ d`` (MP_TAC o AP_TERM ``FILTER p``) THEN
+    RW_TAC std_ss [rich_listTheory.FILTER_APPEND,FILTER, APPEND]);
+
+(*****************************************************************************)
+(* Encoding definitions                                                      *)
+(*****************************************************************************)
+
+val map_fmap_def = Define `map_fmap m1 m2 = L2M o MAP (m1 ## m2) o M2L`;
+
+val all_fmap_def = Define `all_fmap p1 p2 = EVERY (all_pair p1 p2) o M2L`;
+
+val fix_fmap_def = Define `fix_fmap f1 f2 = list (pair I I) o  
+    		   	  	    MINSORT ($<= LEX (K (K T))) o M2L o L2M o sexp_to_list (sexp_to_pair I I) o fix_list (fix_pair f1 f2)`;
+
+val encode_fmap_def = Define `encode_fmap fenc tenc = list (pair fenc tenc) o MINSORT ((inv_image $<= fenc) LEX (K (K T))) o M2L`;
+
+val decode_fmap_def = Define `decode_fmap fdec tdec = L2M o sexp_to_list (sexp_to_pair fdec tdec)`;
+
+val detect_fmap_def = Define `detect_fmap fdet tdet x = 
+    		      	     		  (MAPSET ($<= LEX (K (K T))) o sexp_to_list (sexp_to_pair I I)) x /\ 
+					  (listp (pairp fdet tdet) x)`;
+
+(*****************************************************************************)
+(* Encoding proofs                                                           *)
+(*****************************************************************************)
+
+val o_split = prove(``((a o sexp_to_list f) o list g = a o (sexp_to_list f o list g)) /\
+                      (sexp_to_list f o (list g o b) = (sexp_to_list f o list g) o b)``,
+    METIS_TAC [combinTheory.o_DEF]);
+
+val UNIQL_MAP = store_thm("UNIQL_MAP", ``!f g l. ONE_ONE f /\ uniql l ==> uniql (MAP (f ## g) l)``,
+    RW_TAC std_ss [uniql_def,MAP,MEM,pairTheory.PAIR_MAP,MEM_MAP,ONE_ONE_THM] THEN
+    METIS_TAC [pairTheory.PAIR]);
+
+val PERM_UNIQL = store_thm("PERM_UNIQL", ``!l1 l2. PERM l1 l2 ==> (uniql l1 = uniql l2)``,
+    RW_TAC std_ss [uniql_def,MAP,MEM,ONE_ONE_THM] THEN
+    METIS_TAC [pairTheory.PAIR, MEM_PERM]);
+
+val ONE_ONE_RING = store_thm("ONE_ONE_RING",
+    ``!f g. ONE_ONE (f o g) ==> ONE_ONE g``,
+    RW_TAC std_ss [ONE_ONE_DEF]);
+
+(*****************************************************************************)
+(* ENCDECMAP_FMAP: encode then decode equals map                             *)
+(*****************************************************************************)
+
+val ENCDECMAP_FMAP = store_thm("ENCDECMAP_FMAP", 
+    ``!fdec tdec fenc tenc. ONE_ONE (fdec o fenc) ==> (decode_fmap fdec tdec o encode_fmap fenc tenc = map_fmap (fdec o fenc) (tdec o tenc))``,
+    REWRITE_TAC [decode_fmap_def, encode_fmap_def, o_assoc, map_fmap_def] THEN
+    REWRITE_TAC [o_split, translateTheory.ENCDECMAP_LIST, combinTheory.I_o_ID, quotient_listTheory.LIST_MAP_I, translateTheory.ENCDECMAP_PAIR] THEN
+    RW_TAC std_ss [FUN_EQ_THM] THEN
+    MATCH_MP_TAC L2M_EQ THEN REPEAT CONJ_TAC THEN
+    METIS_TAC [L2M_EQ, UNIQL_MAP, PERM_MAP, PERM_UNIQL, UNIQL_M2L, PERM_MINSORT, UNIQL_MAP, PERM_SETEQ, SETEQ_THM, PERM_SYM]);
+
+(*****************************************************************************)
+(* DECENCFIX_FMAP: decode then encode equals fix                             *)
+(*****************************************************************************)
+
+val RWR = REWRITE_RULE [FUN_EQ_THM, combinTheory.o_THM];
+
+val map_lemma = prove(``!l f g. MAP FST (MAP (f ## g) l) = MAP f (MAP FST l)``,
+    Induct THEN RW_TAC std_ss [MAP, pairTheory.PAIR_MAP]);
+
+val map_eq_sing = prove(``!l f x. (MAP f l = [x]) = ?h. (l = [h]) /\ (x = f h)``,
+    Induct THEN RW_TAC std_ss [MAP, MAP_EQ_NIL] THEN PROVE_TAC []);
+
+val one_one_lemma = prove(``!f. ONE_ONE f ==> !y. $= (f y) o f = $= y``,
+    RW_TAC std_ss [ONE_ONE_THM,FUN_EQ_THM] THEN METIS_TAC []);
+
+val ALL_DISTINCT_MAP = store_thm("ALL_DISTINCT_MAP",
+    ``!l f. ONE_ONE f /\ ALL_DISTINCT l ==> ALL_DISTINCT (MAP f l)``,
+    NTAC 2 (RW_TAC std_ss [ALL_DISTINCT_FILTER, rich_listTheory.FILTER_MAP, map_eq_sing, MEM_MAP, one_one_lemma]));
+
+val M2L_L2M_MAP = store_thm("M2L_L2M_MAP",
+    ``!l f g. ONE_ONE f ==> PERM (M2L (L2M (MAP (f ## g) l))) (MAP (f ## g) (M2L (L2M l)))``,
+    METIS_TAC [ALL_DISTINCT_MAPFST_M2L,ALL_DISTINCT_MAP, map_lemma, ALL_DISTINCT_MAPFST, SETEQ_PERM, M2L_L2M_MAP_SETEQ, ALL_DISTINCT_M2L]);
+
+val MINSORT_M2L_L2M_MAP = store_thm("MINSORT_M2L_L2M_MAP", 
+    ``!l f g. ONE_ONE f ==> (MINSORT ($<= LEX K (K T)) (M2L (L2M (MAP (f ## g) l))) = MINSORT ($<= LEX (K (K T))) (MAP (f ## g) (M2L (L2M l))))``,
+    REPEAT STRIP_TAC THEN MATCH_MP_TAC MAP_FST_DISTINCT_EQ THEN
+    REPEAT CONJ_TAC THEN
+    TRY (MATCH_MP_TAC PERM_SORTED_EQ) THEN
+    TRY (Q.EXISTS_TAC `$<=`) THEN
+    METIS_TAC [M2L_L2M_MAP, PERM_MINSORT, PERM_TRANS,PERM_SYM, PERM_MAP, SORTS_MINSORT, SEXP_LE_TOTAL, 
+               SEXP_LE_TRANSITIVE, TRANSITIVE_K, TOTAL_K, TRANSITIVE_LEX, TOTAL_LEX, SORTS_DEF, SORTED_LEX, 
+               SEXP_LE_ANTISYMMETRIC, ALL_DISTINCT_PERM, ALL_DISTINCT_MAPFST_M2L]);
+
+val MAP_EQ_LENGTH = store_thm("MAP_EQ_LENGTH",
+    ``!l1 l2. (MAP f l1 = MAP g l2) ==> (LENGTH l1 = LENGTH l2)``,
+    METIS_TAC [LENGTH_MAP]);
+
+val MEM_EL_FILTER = store_thm("MEM_EL_FILTER", 
+    ``!f l x. MEM x l ==> ?y. y < LENGTH (FILTER ($= (f x) o f) l) /\ (EL y (FILTER ($= (f x) o f) l) = x)``,
+    GEN_TAC THEN Induct THEN RW_TAC std_ss [FILTER, rich_listTheory.EL_CONS, MEM] THEN RES_TAC THENL [
+       Q.EXISTS_TAC `0`, Q.EXISTS_TAC `SUC y`,ALL_TAC] THEN 
+    RW_TAC arith_ss [LENGTH,EL,HD,TL] THEN
+    METIS_TAC []);
+
+val EL_MAP_FILTER = store_thm("EL_MAP_FITLE",
+    ``!f x. (MAP f l1 = MAP f l2) /\ x < LENGTH l1 /\ (FILTER ($= (f (EL x l1)) o f) l1 = FILTER ($= (f (EL x l2)) o f) l2) ==> (EL x l1 = EL x l2)``,
+    completeInduct_on `LENGTH l1 + LENGTH l2` THEN REPEAT Cases THEN 
+    RW_TAC std_ss [LENGTH, rich_listTheory.EL_CONS, MEM, MAP, FILTER] THEN
+    Cases_on `x` THEN FULL_SIMP_TAC std_ss [rich_listTheory.EL_CONS, EL, HD, TL, list_11] THEN 
+    POP_ASSUM MP_TAC THEN RW_TAC std_ss [list_11] THEN
+    IND_STEP_TAC THEN RW_TAC std_ss [] THEN Q.EXISTS_TAC `f` THEN RW_TAC arith_ss [] THEN METIS_TAC [EL_MAP, LENGTH_MAP]);
+
+val MAP_FST_SND_EQ = store_thm("MAP_FST_SND_EQ",
+    ``!l1 l2. (MAP FST l1 = MAP FST l2) /\ (MAP SND l1 = MAP SND l2) ==> (l1 = l2)``,
+    REPEAT GEN_TAC THEN completeInduct_on `LENGTH l1 + LENGTH l2` THEN REPEAT Cases THEN 
+    RW_TAC std_ss [LENGTH, rich_listTheory.EL_CONS, MEM, MAP, FILTER, pairTheory.PAIR_FST_SND_EQ] THEN
+    IND_STEP_TAC THEN RW_TAC arith_ss []);
+
+val STABLE_FST_EQ = store_thm("STABLE_FST_EQ", 
+    ``!l1 l2. (MAP FST l1 = MAP FST l2) /\ (!x. FILTER ($= x o FST) l1 = FILTER ($= x o FST) l2) ==> (l1 = l2)``,
+    METIS_TAC [EL_MAP_FILTER, EL_MAP, LENGTH_MAP, LIST_EQ_REWRITE,MAP_FST_SND_EQ]);
+
+val SORTED_MAP = store_thm("SORTED_MAP",
+    ``!l f R. transitive R /\ SORTED (inv_image R f) l ==> SORTED R (MAP f l)``,
+    Induct THEN RW_TAC std_ss [SORTED_EQ,SORTED_DEF,MAP,MEM_MAP] THEN
+    REPEAT (POP_ASSUM MP_TAC) THEN RW_TAC std_ss [SORTED_EQ, TRANS_INV, relationTheory.inv_image_def]);
+
+local
+val lemma 
+    = GSYM (GEN_ALL (PULL_RULE (DISCH_ALL (CONJUNCT2 (UNDISCH (SPEC_ALL (PULL_RULE (REWRITE_RULE [STABLE_def] MINSORT_STABLE))))))));
+val sorttac 
+    = RW_TAC std_ss [map_lemma, TRANSITIVE_K, SEXP_LE_ANTISYMMETRIC, SEXP_LE_TRANSITIVE, SEXP_LE_TOTAL, 
+                     REWRITE_RULE [SORTS_DEF] SORTS_MINSORT, TOTAL_K, TOTAL_LEX, TRANSITIVE_LEX, TOTAL_INV, TRANS_INV]
+in
+val MINSORT_PAIRMAP = store_thm("MINSORT_PAIRMAP",
+    ``!f. ONE_ONE f ==> !l g. MINSORT ($<= LEX K (K T)) (MAP (f ## g) l) = MAP (f ## g) (MINSORT (inv_image $<= f LEX K (K T)) l)``,
+    REPEAT STRIP_TAC THEN MATCH_MP_TAC STABLE_FST_EQ THEN REPEAT STRIP_TAC THENL [
+       MATCH_MP_TAC PERM_SORTED_EQ THEN
+       Q.EXISTS_TAC `$<=` THEN sorttac,
+       MATCH_MP_TAC EQ_TRANS THEN 
+       Q.EXISTS_TAC `FILTER ($= x o FST) (MAP (f ## g) l)` THEN CONJ_TAC
+    ] THEN1 METIS_TAC [PERM_MINSORT, PERM_MAP, PERM_SYM, PERM_TRANS, map_lemma] THEN
+    REPEAT (FIRST [MATCH_MP_TAC (PULL_RULE SORTED_LEX) ORELSE MATCH_MP_TAC SORTED_MAP THEN RW_TAC std_ss [SEXP_LE_TRANSITIVE],
+            MATCH_MP_TAC lemma ORELSE MATCH_MP_TAC (GSYM lemma) ORELSE (REWRITE_TAC [rich_listTheory.FILTER_MAP] THEN AP_TERM_TAC)]) THEN
+    TRY (Q.EXISTS_TAC `K (K T)`) THEN sorttac THEN
+    REPEAT (POP_ASSUM MP_TAC) THEN (fn (a,g) => MAP_EVERY (fn b => SPEC_TAC (b,b)) (free_vars g) (a,g)) THEN
+    REPEAT (Cases ORELSE GEN_TAC) THEN RW_TAC std_ss [pairTheory.LEX_DEF,relationTheory.inv_image_def, ONE_ONE_DEF])
+end;
+
+val list_pair_map = prove(``!f g f' g' l. list (pair f g) (MAP (f' ## g') l) = list (pair (f o f') (g o g')) l``,
+    NTAC 4 GEN_TAC THEN Induct THEN RW_TAC std_ss [translateTheory.list_def, translateTheory.pair_def, MAP, pairTheory.PAIR_MAP]);
+
+(*****************************************************************************)
+(* DECENCFIX_FMAP: Decode then encode is fix.                                *)
+(*****************************************************************************)
+
+val DECENCFIX_FMAP = store_thm("DECENCFIX_FMAP",
+    ``!fdec tdec fenc tenc. ONE_ONE (fdec o fenc) ==> (encode_fmap fenc tenc o decode_fmap fdec tdec = fix_fmap (fenc o fdec) (tenc o tdec))``,
+    RW_TAC std_ss [encode_fmap_def,decode_fmap_def,fix_fmap_def,FUN_EQ_THM,GSYM translateTheory.DECENCFIX_LIST,GSYM translateTheory.DECENCFIX_PAIR,
+                  RWR translateTheory.ENCDECMAP_LIST, translateTheory.ENCDECMAP_PAIR] THEN
+    IMP_RES_TAC ONE_ONE_RING THEN
+    RW_TAC std_ss [MINSORT_M2L_L2M_MAP, MINSORT_PAIRMAP, list_pair_map]);
+
+(*****************************************************************************)
+(* MAPID_FMAP: Map identity.                                                 *)
+(*****************************************************************************)
+
+val MAPID_FMAP = store_thm("MAPID_FMAP", 
+    ``map_fmap I I = I``,
+    RW_TAC std_ss [FUN_EQ_THM, map_fmap_def, quotient_pairTheory.PAIR_MAP_I,quotient_listTheory.LIST_MAP_I, L2M_M2L]);
+
+(*****************************************************************************)
+(* FIXID_FMAP: Fix identity.                                                 *)
+(*****************************************************************************)
+
+val FIXID_FMAP = store_thm("FIXID_FMAP",
+    ``(!x. p0 x ==> (f0 x = x)) ∧ (!x. p1 x ==> (f1 x = x)) ==> !x. detect_fmap p0 p1 x ⇒ (fix_fmap f0 f1 x = x)``,
+    RW_TAC std_ss [fix_fmap_def, detect_fmap_def, translateTheory.FIXID_LIST, translateTheory.FIXID_PAIR] THEN
+    SUBGOAL_THEN ``fix_list (fix_pair f0 f1) x = x`` SUBST_ALL_TAC THENL [ALL_TAC,
+        Q.ABBREV_TAC `m = sexp_to_list (sexp_to_pair I I) x` THEN
+        `MINSORT ($<= LEX K (K T)) (M2L (L2M m)) = m` by MATCH_MP_TAC (PULL_RULE M2L_L2M) THEN
+        RW_TAC std_ss [SEXP_LE_TOTAL, SEXP_LE_TRANSITIVE, TRANSITIVE_K, SEXP_LE_ANTISYMMETRIC, SORTS_MINSORT, TRANSITIVE_LEX, TOTAL_LEX, TOTAL_K] THEN
+        POP_ASSUM SUBST_ALL_TAC THEN
+        Q.UNABBREV_TAC `m` THEN
+        RW_TAC std_ss [RWR translateTheory.DECENCFIX_LIST, translateTheory.DECENCFIX_PAIR]] THEN
+    MATCH_MP_TAC (GEN_ALL (PULL_RULE translateTheory.FIXID_LIST)) THEN
+    Q.EXISTS_TAC `pairp p0 p1` THEN RW_TAC std_ss [] THEN MATCH_MP_TAC (GEN_ALL (PULL_RULE translateTheory.FIXID_PAIR)) THEN 
+    METIS_TAC [combinTheory.I_THM,combinTheory.K_THM, translateTheory.GENERAL_DETECT_PAIR]);
+
+val EVERY_PERM = store_thm("EVERY_PERM", ``!l1 l2. PERM l1 l2 ==> (EVERY P l1 = EVERY P l2)``,
+    METIS_TAC [MEM_PERM, EVERY_MEM]);
+
+val INV_LEX_PAIRMAP = store_thm("INV_LEX_PAIRMAP", 
+    ``ONE_ONE f ==> (inv_image (R LEX R') (f ## g) = inv_image R f LEX inv_image R' g)``,
+    RW_TAC std_ss [relationTheory.inv_image_def, pairTheory.LEX_DEF,pairTheory.PAIR_MAP, FUN_EQ_THM] THEN
+    REPEAT (POP_ASSUM MP_TAC) THEN (fn (a,g) => MAP_EVERY (fn b => SPEC_TAC (b,b)) (free_vars g) (a,g)) THEN
+    REPEAT (Cases ORELSE GEN_TAC) THEN RW_TAC std_ss [] THEN
+    METIS_TAC [ONE_ONE_THM]);
+
+val INVIMAGE_K = store_thm("INVIMAGE_K",
+    ``inv_image (K (K T)) x = K (K T)``,
+    RW_TAC std_ss [relationTheory.inv_image_def, pairTheory.LEX_DEF,pairTheory.PAIR_MAP, FUN_EQ_THM] THEN
+    REPEAT (POP_ASSUM MP_TAC) THEN (fn (a,g) => MAP_EVERY (fn b => SPEC_TAC (b,b)) (free_vars g) (a,g)) THEN
+    REPEAT (Cases ORELSE GEN_TAC) THEN RW_TAC std_ss []);
+
+(*****************************************************************************)
+(* ENCDETALL_FMAP: Encoding then detecting equals every                      *)
+(*****************************************************************************)
+
+val ENCDETALL_FMAP = store_thm("ENCDETALL_FMAP",
+    ``!p0 p1 f0 f1. ONE_ONE f0 ==> (detect_fmap p0 p1 o encode_fmap f0 f1 = all_fmap (p0 o f0) (p1 o f1))``,
+    RW_TAC std_ss [FUN_EQ_THM, detect_fmap_def, encode_fmap_def, all_fmap_def, RWR translateTheory.ENCDETALL_LIST, 
+                  all_fmap_def, RWR translateTheory.ENCDECMAP_LIST, translateTheory.ENCDECMAP_PAIR, MAPSET_def, 
+                  translateTheory.ENCDETALL_PAIR, map_lemma] THEN
+    `!Q. EVERY Q (MINSORT (inv_image $<= f0 LEX K (K T)) (M2L x)) = EVERY Q (M2L x)` by MATCH_MP_TAC EVERY_PERM THEN
+    RW_TAC std_ss [PERM_MINSORT, PERM_SYM] THEN
+    MATCH_MP_TAC (DECIDE ``!a b. a ==> (a /\ b = b)``) THEN REPEAT CONJ_TAC THEN
+    MAP_FIRST MATCH_MP_TAC [SORTED_MAP, ALL_DISTINCT_MAP] THEN
+    METIS_TAC [SORTS_MINSORT, SORTS_DEF, TRANSITIVE_LEX, TRANSITIVE_K, SEXP_LE_TRANSITIVE, TOTAL_LEX, TOTAL_K, SEXP_LE_TOTAL, 
+               TOTAL_INV, TRANS_INV, INV_LEX_PAIRMAP, 
+               INVIMAGE_K, ALL_DISTINCT_MAPFST_M2L, PERM_MINSORT, PERM_MAP, PERM_TRANS, PERM_SYM, ALL_DISTINCT_PERM]);
+    
+(*****************************************************************************)
+(* ALLID_FMAP: All identity                                                  *)
+(*****************************************************************************)
+
+val ALLID_FMAP = store_thm("ALLID_FMAP", ``all_fmap (K T) (K T) = K T``,
+    RW_TAC std_ss [all_fmap_def,translateTheory.ALLID_PAIR, translateTheory.ALLID_LIST]);
+
+(*****************************************************************************)
+(* DETECT_DEAD: Detect nil is always true.                                   *)
+(*****************************************************************************)
+
+val DETECTDEAD_FMAP = store_thm("DETECTDEAD_FMAP", ``!p0 p1. detect_fmap p0 p1 nil``,
+    RW_TAC std_ss [detect_fmap_def, translateTheory.sexp_to_list_def, sexpTheory.nil_def, MAPSET_def, 
+       SORTED_DEF, ALL_DISTINCT_THM, MAP, MEM, FILTER, translateTheory.listp_def,translateTheory.pairp_def]);
+
+val MAPSET_CONS = store_thm("MAPSET_CONS", 
+    ``!b a R. MAPSET ($<= LEX (K (K T))) (a::b) ==> MAPSET ($<= LEX (K (K T))) b``,
+    RW_TAC std_ss [MAPSET_def, SORTED_EQ, SEXP_LE_TRANSITIVE, TRANSITIVE_LEX, TRANSITIVE_K, MAP, ALL_DISTINCT]);
+
+(*****************************************************************************)
+(* DETECT_GENERAL_FMAP: An exact map implies any map                         *)
+(*****************************************************************************)
+
+val DETECT_GENERAL_FMAP = store_thm("DETECT_GENERAL_FMAP",
+    ``!p0 p1 x. detect_fmap p0 p1 x ==> detect_fmap (K T) (K T) x``,
+    REWRITE_TAC [detect_fmap_def] THEN
+    NTAC 2 GEN_TAC THEN Induct THEN RW_TAC std_ss [] THEN
+    RW_TAC std_ss [translateTheory.listp_def, translateTheory.pairp_def] THEN
+    FULL_SIMP_TAC std_ss [translateTheory.listp_def,translateTheory.pairp_def, translateTheory.sexp_to_list_def] THEN
+    FIRST_ASSUM MATCH_MP_TAC THEN
+    METIS_TAC [MAPSET_CONS]);
+
+
+(*****************************************************************************)
+(* MAP_COMPOSE: Composition of maps                                          *)
+(* `fmap_map f0 f1 o fmap_map g0 g1 = fmap_map (f0 o g0) (f1 o g1)`          *)
+(* Only needed for types based upon finite maps                              *)
+(*****************************************************************************)
+
+(*****************************************************************************)
+(* ENCMAPENC: Composition of encoding                                        *)
+(* `encode_fmap f0 f1 o map_fmap g0 g1 = encode_fmap (f0 o g0) (f1 o g1)`    *)
+(* Only needed for types based upon finite maps                              *)
+(*****************************************************************************)
 
 val _ = export_theory();
 
